\lesson{18}{Wed Oct 15 2025 15:00}{}

\begin{definition} Newton's Method \leavevmode

    \[
        x_{k+1} = x_{k} - \left[ J_{f}(x_{k})\right]^{-1} f(x_{k})
    \]
    with $ J_{f}(x_{k}) $ nonsingular.

\end{definition}

Newton's method in $ n $ dimensions canno be written as a relaxation iteration in general (comparing to 1D case).

\vspace{2em}
intuition for Newton's methods in nD

    rewrite the Newton's method to 
    \[
        x_{k} - x_{k+1} = \left[ J_{f}(x_{k})\right]^{-1} f(x_{k})
    \]
    \[
        \left[ J_{f}(x_{k})\right](x_{k} - x_{k+1}) = f(x_{k})
    \]

    \[
        \begin{bmatrix}
            \triangledown f_1(x_{k}) \\
            \vdots \\
            \triangledown f_{n}(x_{k})\\
        \end{bmatrix}
        (x_{k} - x_{n+1})
        = 
        \begin{bmatrix}
            f_1(x_{k}) \\
            \vdots \\
            f_{n}(x_{k})\\
        \end{bmatrix}
    \]

    Want to solve for $ x $ in:
    \[
        \triangledown f_{i}(x_{k}) (x_{k} - x) = f_{i}(x_{k})
    \]

\vspace{2em}
\begin{eg}

    $ f: \mathbb{R}^2 \to \mathbb{R}^2 $: $ \{x \in \mathbb{R}^2: \triangledown f_{i}(x) (x - x_{k}) + f_{i}(x_{k})\} = 0 $
    
    Equation for the tangent plane through $ (x_{k}, f_{i}(x_{k})) $:
    \[
        y = \triangledown f_{i}(x_{k}) \cdot (x - x_{k}) + f_{i}(x_{k})
    \]

    The Newton's method is asking for x in $ 0 = \triangledown f_{i}(x_{k}) \cdot (x - x_{k}) + f_{i}(x_{k}) $

\end{eg}


\vspace{2em}
\begin{definition} Taylor Expansion in higher dimension \leavevmode

    \[
        \varphi_{i} (t) = f_{i}((1-t)x + ty) \hspace{2em} f: \mathbb{R}^n \to \mathbb{R} 
    \]
    \[
        \varphi_{i}(z) = \varphi_{i}(z_0) + \varphi_{i}'(z_0)(z - z_0) + \frac{1}{2} \varphi_{i}''(z - z_0)^2 + \cdots 
    \]
    \[
        \varphi_{i}(z) = \varphi_{i}(z_0) + \varphi_{i}(\eta)(z - z_0) \hspace{2em} MVT
    \]
    Set $ z = 1, z_0 = 0 $, 
    \[
        \begin{cases}
            \varphi_1(1) = \varphi_{i}(0) + \varphi_{i}'(\eta)  \hspace{2em} \eta \text{ between 0 and 1}\\
            \varphi_1(1) = \varphi_{i}(0) + \varphi_{i}'(0) + \frac{1}{2} \varphi_{i}''(\eta) \hspace{2em} \eta \text{ between 0 and 1}\\
        \end{cases}
    \]

    \[
        \varphi_{i} = f_1((1-t)x + ty) |_{t = 0} = f_{i}(x)
    \]
    \begin{align*}
        \varphi_{i}'(0) 
        &= \frac{d}{dt}\left[ f_{i}((1-t)x + ty) \right] \\
        &= \sum_{j = 1}^{n} \frac{\partial f_{i}}{\partial x_{j}}\left( (1-t)x + ty \right) |_{t = 0} \frac{d}{dt}\left((1-t)x + ty\right)_j \\
        &= \sum_{j = 1}^{n} \frac{\partial f_{i}}{\partial x_{j}} (x)(y_{j} - x_{j}) = \triangledown f_{i}(x)(y - x) \\
    \end{align*}

    \[
        \varphi_{i}'' = \frac{d}{dt} \sum
    \]

\end{definition}